[itrees] Cleaning and instance

Itree.fst
@@ -81,50 +81,31 @@ let bind #op #s #a #b (x : itree op s a) (f : a -> itree op s b) : itree op s b 
 let loop #op #s a : itree op s a =
   fun p -> Some Tau
 
-(* If we specialised itrees to our needs, we might not need noeq, branching would be known. *)
-// noeq
-// type itree_choice =
-// | Tau_pos : itree_choice
-// | Event_pos : #x : Type -> x -> itree_choice
+(* Monad instance
 
-// type itree_pos = list itree_choice
+   Without GetTrace for now
 
-(* It will be a pain to define a notion of prefix given the noeq *)
-(* let prefix p1 p2 =
-  exists l. p2 = p1 @ l
 *)
 
-// noeq
-// type itree_node (e : Type -> Type) 'r =
-// | Ret : 'r -> itree_node e 'r
-// | Tau : itree_node e 'r
-// | Event : #x : Type -> e x -> itree_node e 'r
+open Common
 
-(* First approach, unguarded. Would need an interface to operate safely. *)
-// type itree1 (e : Type -> Type) (r : Type) =
-//   itree_pos -> option (itree_node e r)
+type cmds = | Openfile | Read | Close
 
-(* Second approach, constraint the tree so that it is consistent. *)
-(*
-type itree2 (e : Type -> Type) (r : Type) =
-  t:(itree_pos -> option (itree_node e r)) {
-    (* Once we reach a terminal node, we can't go futher *)
-    (forall p q. t p = None -> t (p @ q) = None) /\
-    (* Conistency: if a node is Ret, one cannot take the next position *)
-    (forall p q. t p = Some (Ret x) -> t (p @ q) = None) /\
-    (* Conistency for Tau, the only valid position afterward is using Tau_pos *)
-    (forall p. t p = Some Tau -> t (p @ [Tau_pos]) <> None) /\
-    (forall p c. t p = Some Tau -> c <> Tau_pos -> t (p @ [c]) = None) /\
-    (* Conistency for Event, the only valid positions afterward are Event_pos *)
-    (forall p e x. t p = Some (Event e) -> t (p @ [Event_pos x]) <> None) /\
-    (forall p e. t p = Some (Event e) -> t (p @ [Tau_pos]) = None)
-  }
-*)
+unfold let io_args cmd : eqtype =
+  match cmd with
+  | Openfile -> string
+  | Read -> file_descr
+  | Close -> file_descr
 
-(* Third approach, first take a subset of positions and then a map from it to nodes. *)
-(*
-type itree3 (e : Type -> Type) (r : Type) = {
-  pos_sub : itree_pos -> bool { TODO closed by prefix does not contain both p @ Tau_pos and p @ Event_pos, and if p @ Even_pos for one x, then for all x } ;
-  tree : p: itree_pos { pos_sub p } -> itree_node e r
+unfold let io_res cmd : eqtype =
+  match cmd with
+  | Openfile -> file_descr
+  | Read -> string
+  | Close -> unit
+
+let io_op_sig : op_sig cmds = {
+  args = io_args ;
+  res = io_res
 }
-*)
+
+let io a = itree cmds io_op_sig a
